Makefile
@@ -9,23 +9,25 @@ OCAMLFILES= \
 	low/debugType.ml \
 	low/funlist.mli
 
+AT=
+
 %: Makefile.coq phony
-	+make -f Makefile.coq $@
+	${AT}+make -f Makefile.coq $@
 
 all: all_coq all_interp all_html
 
 all_coq: Makefile.coq
-	+make -f Makefile.coq all
+	${AT}+make -f Makefile.coq all
 
 all_html: Makefile.coq
-	+make -f Makefile.coq html
+	${AT}+make -f Makefile.coq html
 
 clean: Makefile.coq clean_interp
-	+make -f Makefile.coq clean
-	rm -f Makefile.coq
+	${AT}+make -f Makefile.coq clean
+	${AT}rm -f Makefile.coq
 
 Makefile.coq: _CoqProject Makefile
-	coq_makefile -f _CoqProject | sed 's/$$(COQCHK) $$(COQCHKFLAGS) $$(COQLIBS)/$$(COQCHK) $$(COQCHKFLAGS) $$(subst -Q,-R,$$(COQLIBS))/' > Makefile.coq
+	${AT}coq_makefile -f _CoqProject | sed 's/$$(COQCHK) $$(COQCHKFLAGS) $$(COQLIBS)/$$(COQCHK) $$(COQCHKFLAGS) $$(subst -Q,-R,$$(COQLIBS))/' > Makefile.coq
 
 _CoqProject: ;
 
@@ -38,42 +40,42 @@ phony: ;
 clean_all: clean clean_tlc
 
 tlc:
-	cd lib/tlc ; make ; cd ../..
+	${AT}cd lib/tlc ; make ; cd ../..
 
 clean_tlc:
-	cd lib/tlc ; make clean ; cd ../..
+	${AT}cd lib/tlc ; make clean ; cd ../..
 
 all_interp: low/runR.native low/runR.d.byte
 
 run: low/runR.native low/initial.state
-	low/runR.native -initial-state low/initial.state
+	${AT}low/runR.native -initial-state low/initial.state
 
 # To launch the program faster through the “make run” command.
 low/initial.state: low/runR.native
-	echo "#save-state low/initial.state\n#quit" | low/runR.native -quiet-output
+	${AT}echo "#save-state low/initial.state\n#quit" | low/runR.native -quiet-output
 
 clean_interp:
-	rm low/runR.native || true
-	rm low/runR.d.byte || true
-	rm -Rf low/_build || true
-	rm -f low.ml{,i} || true
-	rm -f low/low.ml{,i} || true
-	rm -f low/funlist.ml || true
-	# If there if a file low/funlist.v, it would also be a good idea to remove it, but this may removes a human-generated file.
+	${AT}rm low/runR.native || true
+	${AT}rm low/runR.d.byte || true
+	${AT}rm -Rf low/_build || true
+	${AT}rm -f low.ml{,i} || true
+	${AT}rm -f low/low.ml{,i} || true
+	${AT}rm -f low/funlist.ml || true
+	${AT}# If there if a file low/funlist.v, it would also be a good idea to remove it, but this may removes a human-generated file.
 
 low/funlist.ml: low/low.mli low/gen-funlist.pl
-	low/gen-funlist.pl
+	${AT}low/gen-funlist.pl
 
 low/low.ml: low/Extraction.vo
-	mv low.ml low/low.ml || true
+	${AT}mv low.ml low/low.ml || true
 
 low/low.mli: low/Extraction.vo
-	mv low.mli low/low.mli || true
+	${AT}mv low.mli low/low.mli || true
 
 low/runR.native: low/low.ml low/low.mli ${OCAMLFILES} low/funlist.ml
-	cd low ; ocamlbuild -pkg extlib -use-menhir -menhir "menhir --explain" runR.native ; cd ..
+	${AT}cd low ; ocamlbuild -pkg extlib -use-menhir -menhir "menhir --explain" runR.native ; cd ..
 
 # Debug mode
 low/runR.d.byte: low/low.ml low/low.mli ${OCAMLFILES} low/funlist.ml
-	cd low ; ocamlbuild -pkg extlib -use-menhir -menhir "menhir --explain" runR.d.byte ; cd ..
+	${AT}cd low ; ocamlbuild -pkg extlib -use-menhir -menhir "menhir --explain" runR.d.byte ; cd ..
 
